concurrency/scache/CacheInit.i.dfy
@@ -1,0 +1,123 @@
+include "CacheTypes.i.dfy"
+
+module CacheInit(aio: AIO(CacheAIOParams, CacheIfc, CacheSSM)) {
+  import opened IocbStruct
+  import opened AtomicStatusImpl
+  import opened AtomicRefcountImpl
+  import opened AtomicIndexLookupImpl
+  import opened NativeTypes
+  import opened Ptrs
+  import opened Constants
+  import opened GlinearSeq
+  import opened CT = CacheTypes(aio)
+  import opened LinearSequence_i
+  import opened LinearSequence_s
+  import opened CacheHandle
+  import opened Atomics
+  import opened Cells
+  import T = DiskSSMTokens(CacheIfc, CacheSSM)
+  import opened CacheResources
+  import opened GlinearOption
+
+  method split_into_page_size_chunks(glinear pta: PointsToArray<byte>)
+  returns (glinear pta_seq: glseq<PointsToArray<byte>>)
+  requires |pta.s| == CACHE_SIZE * PageSize
+  ensures pta_seq.len() == CACHE_SIZE
+  ensures forall i | 0 <= i < CACHE_SIZE ::
+      pta_seq.has(i)
+        && 0 <= pta.ptr.as_nat() + i * PageSize < 0x1_0000_0000_0000_0000
+        && pta_seq.get(i).ptr == ptr_add(pta.ptr, i as uint64 * PageSize as uint64)
+        && |pta_seq.get(i).s| == PageSize
+
+  method init_cache(glinear init_tok: T.Token)
+  returns (linear c: Cache)
+  requires CacheSSM.Init(init_tok.val)
+  ensures c.Inv()
+  {
+    var data_base_ptr;
+    glinear var data_pta_full;
+    data_base_ptr, data_pta_full := alloc_array_aligned<byte>(
+        CACHE_SIZE as uint64 * PageSize as uint64, 0, PageSize as uint64);
+    glinear var data_pta_seq : glseq<PointsToArray<byte>> :=
+        split_into_page_size_chunks(data_pta_full);
+
+    var iocb_base_ptr;
+    glinear var iocbs;
+    iocb_base_ptr, iocbs := new_iocb_array(NUM_IO_SLOTS as uint64);
+
+    linear var read_refcounts_array := lseq_alloc(RC_WIDTH as uint64 * CACHE_SIZE as uint64);
+    linear var status_idx_array := lseq_alloc(CACHE_SIZE as uint64);
+
+    glinear var empty_seq, dis := split_init(init_tok);
+
+    var i: uint64 := 0;
+    while i < CACHE_SIZE as uint64
+    {
+      linear var cell_idx;
+      glinear var cell_idx_contents;
+      cell_idx, cell_idx_contents := new_cell<int64>(0);
+      glinear var data_pta_seq, data_pta := glseq_take(data_pta_seq, i as nat);
+
+      ghost var key := Key(data_pta.ptr, cell_idx, i as nat);
+
+      glinear var cache_empty;
+      cache_empty, empty_seq := pop_EmptySeq(empty_seq, i as nat, CACHE_SIZE);
+      glinear var handle := CacheEmptyHandle(key, cache_empty, cell_idx_contents, data_pta);
+      glinear var central, rcs := RwLockToken.perform_Init(handle);
+      ghost var rwlock_loc := central.loc;
+
+      linear var atomic_status_atomic := new_atomic(
+          flag_unmapped,
+          AtomicStatusImpl.G(central, glNone),
+          (v, g) => AtomicStatusImpl.state_inv(v, g, key, rwlock_loc),
+          0);
+      linear var atomic_status := AtomicStatus(
+          atomic_status_atomic,
+          rwlock_loc,
+          key);
+
+      linear var status_idx := StatusIdx(atomic_status, cell_idx);
+      lseq_give_inout(inout status_idx_array, i, status_idx);
+
+      var j : uint64 := 0;
+      while j < RC_WIDTH as uint64
+      {
+        glinear var rc;
+        rc, rcs := RwLockToken.pop_rcs(rcs, j as nat, RC_WIDTH);
+        linear var ar_atomic := new_atomic(0, rc,
+            (v, g) => AtomicRefcountImpl.state_inv(v, g, j as nat, rwlock_loc),
+            0);
+        linear var ar := AtomicRefcount(ar_atomic, rwlock_loc);
+
+        // XXX I don't care about the perf of the initialization method, but do note
+        // that the access pattern for writing to this array might be completely awful.
+        lseq_give_inout(inout read_refcounts_array, j * CACHE_SIZE as uint64 + i, ar);
+
+        j := j + 1;
+      }
+
+      dispose_anything(rcs);
+
+      i := i + 1;
+    }
+
+    linear var cache_idx_of_page_array := lseq_alloc(NUM_DISK_PAGES as uint64);
+
+    i := 0;
+    while i < NUM_DISK_PAGES as uint64
+    {
+      glinear var di;
+      di, dis := pop_IdxSeq(dis, i as nat, NUM_DISK_PAGES);
+      linear var ail := new_atomic(-1, di,
+          (v, g) => AtomicIndexLookupImpl.state_inv(v, g, i as nat),
+          0);
+      lseq_give_inout(inout cache_idx_of_page_array, i, ail);
+      i := i + 1;
+    }
+
+    dispose_anything(data_pta_seq);
+    dispose_anything(empty_seq);
+    dispose_anything(dis);
+  }
+
+}
